$\DeclareMathOperator{\sech}{sech}\DeclareMathOperator{\csch}{csch}\DeclareMathOperator{\arcsec}{arcsec}\DeclareMathOperator{\arccot}{arccot}\DeclareMathOperator{\arccsc}{arccosec}\DeclareMathOperator{\arcosh}{arcosh}\DeclareMathOperator{\arsinh}{arsinh}\DeclareMathOperator{\artanh}{artanh}\DeclareMathOperator{\arsech}{arsech}\DeclareMathOperator{\arcsch}{arcosech}\DeclareMathOperator{\arcoth}{arcoth}$
## Integration
$\int{x^n}dx = \frac{x^{n+1}}{n+1} + c$ 
$\int{e^{kx}}dx = \frac{1}{k}e^{kx} + c$  
$\int{\frac {1}{ax+b}}dx = \frac 1a\ln(ax+b) + c$
$\int \ln(x)dx = x\ln(x) - x + c$
$\int{a^x}dx = \frac{a^x}{\ln{a}} + c$  
$\int{\sin kx}dx = -\frac{1}{k}\cos xk + c$  
$\int{\cos kx}dx = \frac{1}{k}\sin kx + c$  
$\int \tan kxdx = \frac 1k \ln|\sec kx| + c$
$\int \csc kxdx = \frac 1k \ln |\csc\space kx - \cot\space kx| + c$
$\int \sec kxdx = \frac 1k \ln |\sec\space kx - \tan\space kx| + c$
$\int \cot kxdx = \frac 1k \ln | \sin\space kx | + c$
$\int{\sec^2x}dx = \tan x + c$  
$\int{\csc^2x}dx = -\cot x + c$  
$\int{\csc x \cot x }dx = -\csc x + c$  
$\int{\sec x \tan x}dx = \sec x + c$
$\int \frac{1}{\sqrt{a^2 - x^2}} = \arcsin(\frac xa)+c$
$\int \frac{1}{x^2 + a^2} = \frac 1a \arctan(\frac xa)+c$
$\int \frac{1}{\sqrt{x^2 - a^2}} = \arcosh(\frac xa)+c$
$\int \frac{1}{\sqrt{x^2 + a^2}} = \arsinh(\frac xa)+c$
$\int \frac{1}{a^2 - x^2} = \frac{1}{2a}\ln|\frac{a+x}{a-x}|+c = \frac 1a\artanh(\frac xa) + c$
$\int \frac{1}{x^2 - a^2} = \frac{1}{2a}\ln|\frac{x-a}{x+a}|+c$


## Differentiation
$\frac{d}{dx}(x^n) = nx^{n-1}$
$\frac{d}{dx}(e^{kx}) = ke^{kx}$
$\frac{d}{dx}(a^x) = \ln(a)*a^x$
$\frac{d}{dx}(\ln{x}) = \frac{1}{x}$
$\frac{d}{dx}(\log_a{x}) = \frac{1}{x\ln a}$
$\frac{d}{dx}(\sin(kx)) = k\cos(kx)$
$\frac{d}{dx}(\cos(kx)) = -k\sin(kx)$
$\frac{d}{dx}(\tan(kx)) = \sec^2(kx)$
$\frac{d}{dx}(\csc(kx)) = -k\csc(kx)\cot(kx)$
$\frac{d}{dx}(\sec(kx)) = k\sec(kx)\tan(kx)$
$\frac{d}{dx}(\cot(kx)) = -k\csc^2(kx)$
$\frac{d}{dx}(\frac 1a \arctan(\frac xa)) = \frac{1}{x^2 + a^2}$
$\frac{d}{dx}(\arcsin(\frac xa)) = \frac{1}{\sqrt{x^2 - a^2}}$


